NewScope

src/Sound/Context.dfy
@@ -10,12 +10,27 @@ module Context {
   function SeqMax(ss: seq<Idx>): Idx 
     ensures forall i <- ss :: i <= SeqMax(ss)
     ensures forall i: nat :: i < |ss| ==> ss[i] <= SeqMax(ss)
+    ensures ss != [] ==> SeqMax(ss) in ss
   {
     if ss == [] then 
       0 
     else
       assert ss == [ss[0]] + (ss[1..]);
       max(ss[0], SeqMax(ss[1..]))
+  }
+
+  lemma MaxInsertLemma(ss: seq<Idx>, i: nat, x: Idx)
+    requires forall s <- ss :: s < x
+    requires i < |ss|
+    ensures SeqMax(ss[i := x]) == x 
+  {
+    assert forall x :: x in ss[1..] ==> x in ss;
+    assert ss[0] in ss;
+    if ss != [] {
+      if i != 0 {
+        MaxInsertLemma(ss[1..], i - 1, x);
+      }
+    }
   }
 
   datatype Context = Context(
@@ -108,9 +123,8 @@ module Context {
       ensures SeqMax(incarnation) + 1 == SeqMax(context.incarnation)
     {
       var v' := FreshIdx();
+      MaxInsertLemma(incarnation, v, v');
       var ctx' := ctx + [Eq(BVar(v'), Substitute(e))];
-      // FVarsEqLemma(Var(v'), Substitute(e));
-      // FVarsConjUnionLemma(ctx, [Eq(Var(v'), Substitute(e))]);
       var incarnation' := incarnation[v := v'];
       context := Context(ctx', incarnation');
       vNew := v';
@@ -174,8 +188,8 @@ module Context {
     lemma ForallPush(s1: State, s2: State, e1: Expr, e2: Expr)
       requires e1.IsDefinedOn(|s1| + 1)
       requires e2.IsDefinedOn(|s2| + 1)
-      requires forall b: bool :: s1.Update(b).Eval(e1) == s2.Update(b).Eval(e2)
-      ensures (forall b: bool :: s1.Update(b).Eval(e1)) == (forall b: bool :: s2.Update(b).Eval(e2))
+      requires forall b: bool :: s1.Update([b]).Eval(e1) == s2.Update([b]).Eval(e2)
+      ensures (forall b: bool :: s1.Update([b]).Eval(e1)) == (forall b: bool :: s2.Update([b]).Eval(e2))
     {  }
 
     lemma AdjustStateSubstituteIdxLemma(s: State, e: Expr, i: Idx)
@@ -190,13 +204,13 @@ module Context {
       case Forall(v, body) =>
         SubstituteIdxIsDefinedOnLemma(e, i, |s|);
         assert forall b: bool :: 
-          ((s[..i] + AdjustState(s[i..])).Update(b)).Eval(body) == 
-          (s.Update(b)).Eval(SubstituteIdx(body, i + 1)) by {
+          ((s[..i] + AdjustState(s[i..])).Update([b])).Eval(body) == 
+          (s.Update([b])).Eval(SubstituteIdx(body, i + 1)) by {
           forall b: bool 
-            ensures ((s[..i] + AdjustState(s[i..])).Update(b)).Eval(body) == (s.Update(b)).Eval(SubstituteIdx(body, i + 1)) {
+            ensures ((s[..i] + AdjustState(s[i..])).Update([b])).Eval(body) == (s.Update([b])).Eval(SubstituteIdx(body, i + 1)) {
             assert ([b] + s)[..i+1] == [b] + s[..i];
             assert ([b] + s)[i+1..] == s[i..];
-            assert ((s[..i] + AdjustState(s[i..])).Update(b)) == (([b] + s)[..i+1] + AdjustState(([b] + s)[i+1..]));
+            assert ((s[..i] + AdjustState(s[i..])).Update([b])) == (([b] + s)[..i+1] + AdjustState(([b] + s)[i+1..]));
             AdjustStateSubstituteIdxLemma([b] + s, body, i + 1);
           }
         }
@@ -218,239 +232,3 @@ module Context {
 
   }
 }
-
-  /*datatype Context = Context(P
-    ctx: seq<Expr>, 
-    incarnation: seq<Variable>,
-    bVars: set<Variable>) 
-  {
-
-    /*ghost const Models : iset<State> := iset st: State | IsSatisfiedOn(st)
-    // Q: is it correct way to set a trigger?
-    ghost const AdjustedModels : iset<State> := 
-      iset st: State | exists st' <- Models {:InAdjustedModelsLemma(st')} :: AdjustState(st') == st
-
-    lemma InAdjustedModelsLemma(st: State, st': State)
-      requires IsSatisfiedOn(st')
-      requires st == AdjustState(st')
-      ensures st in AdjustedModels
-    {
-
-    }
-
-    function CtxFVars(): set<Variable> 
-      ensures CtxFVars() == Conj(ctx).FVars()
-      ensures forall e <- ctx :: e.FVars() <= CtxFVars()
-      decreases ctx
-    {
-      if ctx == [] then {} else ctx[0].FVars() + Context(ctx[1..], incarnation, bVars).CtxFVars()
-    }
-
-    function FVars(): set<Variable> 
-    {
-      CtxFVars() + incarnation.Values
-    }
-
-    ghost predicate Valid() 
-    {
-      forall b <- bVars :: b !in incarnation.Values
-    }
-
-    function FreshVar(): Variable
-      ensures {:axiom} FreshVar() !in incarnation.Keys
-      ensures {:axiom} FreshVar() !in bVars
-      ensures {:axiom} FreshVar() !in FVars()
-
-
-    function AdjustState(s: State): State
-      requires incarnation.Values <= s.Keys
-    { 
-      map x: Variable | x in incarnation.Keys :: s[incarnation[x]] 
-    }
-
-    function Substitute(e: Expr): Expr 
-      decreases e
-    {
-      match e
-      case BConst(bvalue) => e
-      case Var(v) =>
-        if v in incarnation then  
-          Var(incarnation[v]) 
-        else e
-      case And(e0, e1) => 
-        And(Substitute(e0), Substitute(e1))
-      case Or(e0, e1) => 
-        Or(Substitute(e0), Substitute(e1))
-      case Not(e) => 
-        Not(Substitute(e))
-      case Implies(e0, e1) => 
-        Implies(Substitute(e0), Substitute(e1))
-      case Forall(v, body) => 
-        Forall(v, Context(ctx, incarnation[v := v], bVars).Substitute(body))
-    }
-
-    function MkEntailment(e: Expr): Expr 
-    {
-      Implies(Conj(ctx), Substitute(e))
-    }
-
-
-    function Add(e: Expr): Context
-      requires Valid()
-      requires e.IsDefinedOn(incarnation.Keys)
-      ensures Add(e).Valid()
-    {
-      ghost var ctx' := ctx;
-      var ctx := ctx + [Substitute(e)];
-      FVarsConjUnionLemma(ctx', [Substitute(e)]);
-      Context(ctx, incarnation, bVars)
-    }
-
-    method AddEq(v: Variable, e: Expr) returns (ghost vNew: Variable, context: Context)
-      requires v in incarnation.Keys
-      requires Valid()
-      ensures context.Valid()
-      ensures incarnation.Keys == context.incarnation.Keys
-      ensures ctx + [Eq(Var(vNew), Substitute(e))] == context.ctx
-      ensures incarnation[v := vNew] == context.incarnation
-      ensures bVars == context.bVars
-      ensures vNew !in incarnation.Keys
-      ensures vNew !in bVars
-      ensures vNew !in FVars()
-    {
-      var v' := FreshVar();
-      var ctx' := ctx + [Eq(Var(v'), Substitute(e))];
-      FVarsEqLemma(Var(v'), Substitute(e));
-      FVarsConjUnionLemma(ctx, [Eq(Var(v'), Substitute(e))]);
-      var incarnation' := incarnation[v := v'];
-      context := Context(ctx', incarnation', bVars);
-      vNew := v';
-    }
-    
-    method AddVar(v: Variable) returns (ghost vNew: Variable, context: Context)
-      requires Valid()
-      ensures context.Valid()
-
-      ensures context.incarnation == incarnation[v := vNew]
-      ensures context.ctx         == ctx
-      ensures context.bVars       == bVars
-
-      ensures vNew !in incarnation.Keys
-      ensures vNew !in bVars
-      ensures vNew !in FVars()
-    {
-      var v' := FreshVar();
-      var incarnation' := incarnation[v := v'];
-      context := Context(ctx, incarnation', bVars);
-      vNew := v';
-    }
-    
-    ghost predicate IsDefinedOn(s: set<Variable>) 
-    {
-      FVars() <= s
-    }
-
-    lemma FVarsLemma(s: set<Variable>)
-      requires IsDefinedOn(s)
-      ensures forall e <- ctx :: e.IsDefinedOn(s)
-    {  }
-
-    ghost predicate IsSatisfiedOn(s: State) 
-    {
-      && IsDefinedOn(s.Keys) 
-      && incarnation.Values <= s.Keys
-      && forall e <- ctx :: s.Eval(e)
-    }
-
-    ghost predicate Entails(e: Expr) 
-    {
-      forall s: State ::  
-        e.IsDefinedOn(s.Keys) && IsSatisfiedOn(s) ==> s.Eval(e)
-    }
-
-    lemma SubstituteIsDefinedOnLemma(e: Expr)
-      requires e.IsDefinedOn(incarnation.Keys)
-      ensures Substitute(e).IsDefinedOn(incarnation.Values)
-      decreases e
-    {
-      assert e.FVars() <= incarnation.Keys;
-      match e 
-      case Forall(v, body) => Context(ctx, incarnation[v := v], bVars).SubstituteIsDefinedOnLemma(body);
-      case _ => 
-    }
-
-
-    lemma AdjustStateSubstituteLemma'(s: State, e: Expr)
-      requires forall b <- e.BVars(), x <- incarnation.Keys :: incarnation[x] == b ==> x == b
-      requires e.IsDefinedOn(incarnation.Keys)
-      requires incarnation.Values <= s.Keys
-      ensures Substitute(e).IsDefinedOn(s.Keys)
-      ensures (
-        SubstituteIsDefinedOnLemma(e); 
-        AdjustState(s).Eval(e) == s.Eval(Substitute(e)))
-      decreases e
-    {
-      match e 
-      case Forall(v, body) => 
-        var ctx' := Context(ctx, incarnation[v := v], bVars);
-        SubstituteIsDefinedOnLemma(Forall(v, body)); 
-        assert forall b: bool :: 
-          AdjustState(s).Update(v, b).Eval(body) == 
-          s.Update(v, b).Eval(ctx'.Substitute(body)) by 
-        {
-          forall b: bool 
-            ensures AdjustState(s).Update(v, b).Eval(body) == 
-              s.Update(v, b).Eval(ctx'.Substitute(body)) 
-            {
-              assert AdjustState(s)[v:=b] == ctx'.AdjustState(s[v:=b]) by {
-                assert AdjustState(s)[v:=b].Keys == ctx'.AdjustState(s[v:=b]).Keys;
-                forall x: Variable {:trigger} | x in AdjustState(s)[v:=b].Keys
-                  ensures AdjustState(s)[v:=b][x] == ctx'.AdjustState(s[v:=b])[x] {
-                  if x != v {
-                    if incarnation[x] == v {
-                      assert v in e.BVars();
-                    }
-                  }
-                }
-              }
-              assert forall b <- body.BVars() {:trigger}, x <- incarnation[v:=v].Keys :: 
-                incarnation[v:=v][x] == b ==> x == b by 
-              {
-                forall b <- body.BVars() {:trigger}, x <- incarnation[v:=v].Keys
-                ensures incarnation[v:=v][x] == b ==> x == b {
-                  if x != v {
-                    assert e.BVars() == body.BVars() + {v};
-                  }
-                }
-              }
-              ctx'.AdjustStateSubstituteLemma'(s.Update(v, b), body);
-            }
-        }
-      case Var(v) =>
-      case BConst(bvalue) =>
-      case Not(ne) => 
-        assert ne.BVars() == e.BVars();
-      case And(e0, e1) => 
-        assert e0.BVars() <= e.BVars(); 
-        assert e1.BVars() <= e.BVars();
-      case Or(e0, e1) => 
-        assert e0.BVars() <= e.BVars(); 
-        assert e1.BVars() <= e.BVars();
-      case Implies(e0, e1) => 
-        assert e0.BVars() <= e.BVars(); 
-        assert e1.BVars() <= e.BVars();
-    }
-
-    lemma AdjustStateSubstituteLemma(s: State, e: Expr)
-      requires e.BVars() <= bVars
-      requires Valid()
-      requires e.IsDefinedOn(incarnation.Keys)
-      requires IsDefinedOn(s.Keys)
-      ensures Substitute(e).IsDefinedOn(s.Keys)
-      ensures (
-        SubstituteIsDefinedOnLemma(e); 
-        AdjustState(s).Eval(e) == s.Eval(Substitute(e)))
-    { AdjustStateSubstituteLemma'(s, e); }*/
-  }
-
-}*/
